Use handle in examples #177

base/coq/Free/Verification/SharingHandlerTests.v
@@ -1,6 +1,7 @@
 (** * Test module for sharing handlers. *)
 
 From Base Require Import Free.
+From Base Require Import Free.HandlerInstances.
 From Base Require Import Free.Instance.Comb.
 From Base Require Import Free.Instance.Identity.
 From Base Require Import Free.Instance.Maybe.
@@ -16,27 +17,6 @@ From Base Require Import Free.Util.Search.
 
 Require Import Lists.List.
 Import List.ListNotations.
-
-(* Shortcut to evaluate a non-deterministic program to a result list.
-   list. *)
-Definition evalND {A : Type} p
-:= @collectVals A (run (runChoice (runNDSharing (0,0) p))).
-
-(* Shortcut to evaluate a traced program to a result and a list of logged 
-   messages. *)
-Definition evalTracing {A : Type} p 
-:= @collectMessages A (run (runTracing (runTraceSharing (0,0) p))).
-
-(* Shortcut to evaluate a non-deterministic partial program to a result 
-   list. *)
-Definition evalNDM {A : Type} p
-:= @collectVals (option A) (run (runChoice (runNDSharing (0,0) (runMaybe p)))).
-
-(* Shortcut to evaluate a traced partial pro gram to a result and a list 
-   of logged messages. *)
-Definition evalTraceM {A : Type} p
-:= @collectMessages (option A) 
-   (run (runTracing (runTraceSharing (0,0) (runMaybe p)))).
 
 Section SecData.
 
@@ -219,7 +199,7 @@ Notation "'orBool_'" := (orBool _ _).
 = 0+0 ? 0+1 ? 1+0 ? 1+1
 = 0 ? 1 ? 1 ? 2
 *)
-Example exAddNoSharingND : evalND (nf (double addInteger_ coin))
+Example exAddNoSharingND : handle (double addInteger_ coin)
                            = [0%Z;1%Z;1%Z;2%Z].
 Proof. constructor. Qed.
 
@@ -228,7 +208,7 @@ trace "One" 1 + trace "One" 1
 => The message should be logged twice and the result should be 2.
 *)
 Example exAddNoSharingTrace 
-: evalTracing (nf (double addInteger_ traceOne))
+: handle (double addInteger_ traceOne)
   = (2%Z,["One"%string;"One"%string]).
 Proof. constructor. Qed.
 
@@ -239,7 +219,7 @@ Proof. constructor. Qed.
 = true ? true ? false
 *)
 Example exOrNDNoSharing 
- : evalND (nf (double orBool_ coinB)) = [true;true;false].
+ : handle (double orBool_ coinB) = [true;true;false].
 Proof. constructor. Qed.
 
 (*
@@ -248,7 +228,7 @@ Proof. constructor. Qed.
    message should be logged only once.
 *)
 Example exOrTrueTracingNoSharing 
- : evalTracing (nf (double orBool_ traceTrue))
+ : handle (double orBool_ traceTrue)
    = (true,["True"%string]).
 Proof. constructor. Qed.
 
@@ -258,7 +238,7 @@ Proof. constructor. Qed.
    should be logged twice.
 *)
 Example exOrFalseTracingNoSharing 
- : evalTracing (nf (double orBool_ traceFalse))
+ : handle (double orBool_ traceFalse)
    = (false,["False"%string;"False"%string]).
 Proof. constructor. Qed.
 
@@ -268,7 +248,7 @@ Proof. constructor. Qed.
    should be logged.
 *)
 Example exOrMixedTracingNoSharing
- : evalTracing (nf (orBool_ traceFalse traceTrue))
+ : handle (orBool_ traceFalse traceTrue)
    = (true,["False"%string;"True"%string]).
 Proof. constructor. Qed.
 
@@ -280,7 +260,7 @@ Proof. constructor. Qed.
 = Nothing ? Nothing ? Just 2
 *)
 Example exNDMNoSharing
- : evalNDM (nf (double addInteger_ coinM)) = [None;None;Some 2%Z].
+ : handle (double addInteger_ coinM) = [None;None;Some 2%Z].
 Proof. constructor. Qed.
 
 (* 
@@ -289,7 +269,7 @@ trace "Nothing" Nothing + trace "Nothing" Nothing
    only be logged once and the result should be Nothing (i.e. None in Coq).
 *)
 Example exTraceNothingNoSharing
- : evalTraceM (nf (double addInteger_ traceNothing))
+ : handle (double addInteger_ traceNothing)
    = (None,["Nothing"%string]).
 Proof. constructor. Qed.
 
@@ -299,7 +279,7 @@ trace "Just 1" (Just 1) + trace "Just 1" (Just 1)
    result should be Just 2 (Some 2 in Coq).
 *)
 Example exTraceJustNoSharing
- : evalTraceM (nf (double addInteger_ traceJust))
+ : handle (double addInteger_ traceJust)
    = (Some 2%Z,["Just 1"%string;"Just 1"%string]).
 Proof. constructor. Qed.
 
@@ -312,8 +292,8 @@ in sx + sx
 = 0+0 ? 1+1
 = 0 ? 2
 *)
-Example exAddSharingND : evalND (nf (doubleShared Cbneed_
-  addInteger_ coin))
+Example exAddSharingND : handle (doubleShared Cbneed_
+  addInteger_ coin)
   = [0%Z;2%Z].
 Proof. constructor. Qed.
 
@@ -323,7 +303,7 @@ in sx + sx
 => The message should be logged once and the result should be 2.
 *)
 Example exAddSharingTrace 
- : evalTracing (nf (doubleShared Cbneed_ addInteger_ traceOne))
+ : handle (doubleShared Cbneed_ addInteger_ traceOne)
  = (2%Z,["One"%string]).
 Proof. constructor. Qed.
 
@@ -334,7 +314,7 @@ in sx or sx
 = true ? false
 *)
 Example exOrNDSharing
- : evalND (nf (doubleShared Cbneed_ orBool_ coinB)) = [true;false].
+ : handle (doubleShared Cbneed_ orBool_ coinB) = [true;false].
 Proof. constructor. Qed.
 
 (*
@@ -344,7 +324,7 @@ in sx or sx
    The message should be logged once and the result should be true.
 *)
 Example exOrTrueTraceSharing
- : evalTracing (nf (doubleShared Cbneed_ orBool_ traceTrue))
+ : handle (doubleShared Cbneed_ orBool_ traceTrue)
    = (true,["True"%string]).
 Proof. constructor. Qed.
 
@@ -355,15 +335,15 @@ in sx or sx
 only be logged once and the result should be false.
 *)
 Example exOrFalseTraceSharing
- : evalTracing (nf (doubleShared Cbneed_ orBool_ traceFalse))
+ : handle (doubleShared Cbneed_ orBool_ traceFalse)
    = (false,["False"%string]).
 Proof. constructor. Qed.
 
 (* traceFalse is shared, but does not occur more than once. 
    Therefore, sharing should make no difference here. *)
 Example exOrMixedTraceSharing
- : evalTracing (nf (share traceFalse >>= fun sx => 
-                (orBool_ sx traceTrue)))
+ : handle (share traceFalse >>= fun sx => 
+                (orBool_ sx traceTrue))
    = (true,["False"%string;"True"%string]).
 Proof. constructor. Qed.
 
@@ -374,7 +354,7 @@ in sx + sx
 = Nothing ? Just 2
 *)
 Example exNDMSharing
- : evalNDM (nf (doubleShared Cbneed_ addInteger_ coinM))
+ : handle (doubleShared Cbneed_ addInteger_ coinM)
    = [None;Some 2%Z].
 Proof. constructor. Qed.
 
@@ -385,7 +365,7 @@ in sx + sx
    due to >>=.
 *)
 Example exTraceNothingSharing
- : evalTraceM (nf (doubleShared Cbneed_ addInteger_ traceNothing))
+ : handle (doubleShared Cbneed_ addInteger_ traceNothing)
    = (None,["Nothing"%string]).
 Proof. constructor. Qed.
 
@@ -396,7 +376,7 @@ in sx + sx
    should be Some 2.
 *)
 Example exTraceJustSharing
- : evalTraceM (nf (doubleShared Cbneed_ addInteger_ traceJust))
+ : handle (doubleShared Cbneed_ addInteger_ traceJust)
    = (Some 2%Z,["Just 1"%string]).
 Proof. constructor. Qed.
 
@@ -409,9 +389,9 @@ in sy + sy
 = (0+0)+(0+0) ? (1+1)+(1+1) 
 = 0 ? 4 
 *)
-Example exAddNestedSharingND : evalND (nf (doubleSharedNested Cbneed_
+Example exAddNestedSharingND : handle (doubleSharedNested Cbneed_
                                                           addInteger_ 
-                                                          coin))
+                                                          coin)
                                = [0%Z;4%Z].
 Proof. constructor. Qed.
 
@@ -422,7 +402,7 @@ in sy + sy
 => The message should only be logged once and the result should be 4. 
 *)
 Example exAddNestedSharingTrace 
- : evalTracing (nf (doubleSharedNested Cbneed_ addInteger_ traceOne))
+ : handle (doubleSharedNested Cbneed_ addInteger_ traceOne)
    = (4%Z,["One"%string]).
 Proof. constructor. Qed.
 
@@ -433,7 +413,7 @@ in sy or sy
 = true ? false
 *)
 Example exOrNestedSharingND
- : evalND (nf (doubleSharedNested Cbneed_ orBool_ coinB))
+ : handle (doubleSharedNested Cbneed_ orBool_ coinB)
    = [true;false].
 Proof. constructor. Qed.
 
@@ -445,7 +425,7 @@ in sy or sy
    and the result should be true.
 *)
 Example exOrNestedTrueTracing 
- : evalTracing (nf (doubleSharedNested Cbneed_ orBool_ traceTrue))
+ : handle (doubleSharedNested Cbneed_ orBool_ traceTrue)
    = (true,["True"%string]).
 Proof. constructor. Qed.
 
@@ -457,7 +437,7 @@ in sy or sy
    and the result should be false.
 *)
 Example exOrNestedFalseTracing
- : evalTracing (nf (doubleSharedNested Cbneed_ orBool_ traceFalse))
+ : handle (doubleSharedNested Cbneed_ orBool_ traceFalse)
    = (false, ["False"%string]).
 Proof. constructor. Qed.
 
@@ -472,7 +452,7 @@ in sy + sz
 = 0 ? 1 ? 2 ? 3
 *)
 Example exAddClashSharingND
- : evalND (nf (doubleSharedClash Cbneed_ addInteger_ coin coin))
+ : handle (doubleSharedClash Cbneed_ addInteger_ coin coin)
    = [0%Z;1%Z;2%Z;3%Z].
 Proof. constructor. Qed.
 
@@ -484,8 +464,8 @@ in sy + sz
 => The message should be logged twice and the result should be 3.
 *)
 Example exAddClashSharingTracing
- : evalTracing (nf (doubleSharedClash Cbneed_ addInteger_
-                                  traceOne traceOne))
+ : handle (doubleSharedClash Cbneed_ addInteger_
+                                  traceOne traceOne)
    = (3%Z,["One"%string;"One"%string]).
 Proof. constructor. Qed.
 
@@ -499,7 +479,7 @@ in sy or sz
 = true ? true ? false
 *)
 Example exOrClashSharingND
- : evalND (nf (doubleSharedClash Cbneed_ orBool_ coinB coinB))
+ : handle (doubleSharedClash Cbneed_ orBool_ coinB coinB)
    = [true;true;false].
 Proof. constructor. Qed.
 
@@ -512,8 +492,8 @@ in sy or sz
    result should be true.
 *)
 Example exOrClashTrueTracing
- : evalTracing (nf (doubleSharedClash Cbneed_ orBool_
-                                  traceTrue traceTrue))
+ : handle (doubleSharedClash Cbneed_ orBool_
+                                  traceTrue traceTrue)
    = (true,["True"%string]).
 Proof. constructor. Qed.
 
@@ -527,8 +507,8 @@ in sy or sz
    be logged twice in total and the result should be false.
 *)
 Example exOrClashFalseTracing
- : evalTracing (nf (doubleSharedClash Cbneed_ orBool_
-                                  traceFalse traceFalse))
+ : handle (doubleSharedClash Cbneed_ orBool_
+                                  traceFalse traceFalse)
    = (false,["False"%string;"False"%string]).
 Proof. constructor. Qed.
 
@@ -544,9 +524,9 @@ in sx + (sy + (sz + 1))
   ? (1 + (1+1 + ((1+1 + 1) + 1)))
 = 4 ? 5 ? 6 ? 7
 *)
-Example exAddRecSharingND : evalND (nf (doubleSharedRec Cbneed_
+Example exAddRecSharingND : handle (doubleSharedRec Cbneed_
                                                     addInteger_
-                                                    coin coin 1%Z))
+                                                    coin coin 1%Z)
                             = [4%Z;5%Z;6%Z;7%Z].
 Proof. constructor. Qed.
 
@@ -561,8 +541,8 @@ in sx + (sy + (sz + 1))
    final value should be 1 + 2 + 3 + 1 = 7.
 *)
 Example exAddRecSharingTracing
- : evalTracing (nf (doubleSharedRec Cbneed_ addInteger_
-                                traceOne traceOne 1%Z))
+ : handle (doubleSharedRec Cbneed_ addInteger_
+                                traceOne traceOne 1%Z)
    = (7%Z,["One"%string;"One"%string]).
 Proof. constructor. Qed.
 
@@ -574,7 +554,7 @@ in sx or (sy or (sz or true))
 = true (due to non-strictness)
 *)
 Example exOrRecSharingNDTrue
- : evalND (nf (doubleSharedRec Cbneed_ orBool_ coinB coinB true))
+ : handle (doubleSharedRec Cbneed_ orBool_ coinB coinB true)
    = [true].
 Proof. constructor. Qed.
 
@@ -597,7 +577,7 @@ in sx or (sy or (sz or false))
 = true ? true ? false
 *)
 Example exOrRecSharingNDFalse
- : evalND (nf ((doubleSharedRec Cbneed_ orBool_ coinB coinB false)))
+ : handle ((doubleSharedRec Cbneed_ orBool_ coinB coinB false))
    = [true;true;false].
 Proof. constructor. Qed.
 
@@ -610,8 +590,8 @@ in sx or (sy or (sz or false))
    be logged once and the result should be true.
 *)
 Example exOrRecTrueTracing
- : evalTracing (nf (doubleSharedRec Cbneed_ orBool_
-                                traceTrue traceTrue false))
+ : handle (doubleSharedRec Cbneed_ orBool_
+                                traceTrue traceTrue false)
    = (true,["True"%string]).
 Proof. constructor. Qed.
 
@@ -625,8 +605,8 @@ in sx or (sy or (sz or false))
    be false.
 *)
 Example exOrRecFalseTracing
- : evalTracing (nf (doubleSharedRec Cbneed_ orBool_
-                                traceFalse traceFalse false))
+ : handle (doubleSharedRec Cbneed_ orBool_
+                                traceFalse traceFalse false)
    = (false,["False"%string;"False"%string]).
 Proof. constructor. Qed.
 
@@ -641,7 +621,7 @@ in fst sx + fst sx
 = 0 ? 2
 *)
 Example exAddDeepPairND 
- : evalND (nf (doubleDeepSharedPair Cbneed_ addInteger_ coinPair))
+ : handle (doubleDeepSharedPair Cbneed_ addInteger_ coinPair)
   = [0%Z;2%Z].
 Proof. constructor. Qed.
 
@@ -651,8 +631,8 @@ in head sx + head sx
 = 0 ? 2
 *)
 Example exAddDeepListND
- : evalND (nf 
-  (doubleDeepSharedList (PartialLifted ND.Shape ND.Pos _ _ ND.Partial) Cbneed_ addInteger_ coinList))
+ : handle
+  (doubleDeepSharedList (PartialLifted ND.Shape ND.Pos _ _ ND.Partial) Cbneed_ addInteger_ coinList)
  = [0%Z;2%Z].
 Proof. constructor. Qed.
 
@@ -664,7 +644,7 @@ in fst sx + fst sx
    should not be logged and the first should be shared and thus logged once. 
 *)
 Example exAddDeepPairTrace
- : evalTracing (nf (doubleDeepSharedPair Cbneed_ addInteger_ tracePair))
+ : handle (doubleDeepSharedPair Cbneed_ addInteger_ tracePair)
   = (0%Z, ["0"%string]).
 Proof. constructor. Qed.
 
@@ -678,7 +658,7 @@ in head sx + head sx
    should be Some 0 instead of simply 0.
 *)
 Example exAddDeepListTrace
- : evalTraceM (nf 
-   (doubleDeepSharedList (PartialLifted Maybe.Shape Maybe.Pos _ _ Maybe.Partial) Cbneed_ addInteger_ traceList))
+ : handle 
+   (doubleDeepSharedList (PartialLifted Maybe.Shape Maybe.Pos _ _ Maybe.Partial) Cbneed_ addInteger_ traceList)
   = (Some 0%Z, ["0"%string]).
 Proof. constructor. Qed.
